add boundary/break forms

Capless/Term.lean
@@ -17,16 +17,18 @@ inductive Term : Nat -> Nat -> Nat -> Type where
 | letex : Term n m k -> Term (n+1) m (k+1) -> Term n m k
 | bindt : SType n m k -> Term n (m+1) k -> Term n m k
 | bindc : CaptureSet n k -> Term n m (k+1) -> Term n m k
+| boundary : SType n m k -> Term (n+1) m (k+1) -> Term n m k
 | unbox : CaptureSet n k -> Fin n -> Term n m k
 
 notation:50 "λ(x:" T ")" t => Term.lam T t
 notation:50 "λ[X<:" S "]" t => Term.tlam S t
 notation:50 "λ[c]" t => Term.clam t
 notation:50 C " o- " x => Term.unbox C x
-notation:40 "let x=" t "in" u => Term.letin t u
-notation:40 "let (c,x)=" t "in" u => Term.letex t u
-notation:40 "let X=" S "in" t => Term.bindt S t
-notation:40 "let c=" C "in" t => Term.bindc C t
+notation:40 "let x=" t " in " u => Term.letin t u
+notation:40 "let (c,x)=" t " in " u => Term.letex t u
+notation:40 "let X=" S " in " t => Term.bindt S t
+notation:40 "let c=" C " in " t => Term.bindc C t
+notation:40 "boundary:" S " in " t => Term.boundary S t
 
 inductive Term.IsValue : Term n m k -> Prop where
 | lam : Term.IsValue (lam E t)
@@ -51,6 +53,7 @@ def Term.rename (t : Term n m k) (f : FinFun n n') : Term n' m k :=
   | Term.bindt S t => Term.bindt (S.rename f) (t.rename f)
   | Term.bindc c t => Term.bindc (c.rename f) (t.rename f)
   | Term.unbox c x => Term.unbox (c.rename f) (f x)
+  | Term.boundary S t => Term.boundary (S.rename f) (t.rename f.ext)
 
 def Term.trename (t : Term n m k) (f : FinFun m m') : Term n m' k :=
   match t with
@@ -68,6 +71,7 @@ def Term.trename (t : Term n m k) (f : FinFun m m') : Term n m' k :=
   | Term.bindt S t => Term.bindt (S.trename f) (t.trename f.ext)
   | Term.bindc c t => Term.bindc c (t.trename f)
   | Term.unbox c x => Term.unbox c x
+  | Term.boundary S t => Term.boundary (S.trename f) (t.trename f)
 
 def Term.crename (t : Term n m k) (f : FinFun k k') : Term n m k' :=
   match t with
@@ -85,6 +89,7 @@ def Term.crename (t : Term n m k) (f : FinFun k k') : Term n m k' :=
   | Term.bindt S t => Term.bindt (S.crename f) (t.crename f)
   | Term.bindc c t => Term.bindc (c.crename f) (t.crename f.ext)
   | Term.unbox c x => Term.unbox (c.crename f) x
+  | Term.boundary S t => Term.boundary (S.crename f) (t.crename f.ext)
 
 theorem IsValue.rename_l' {t : Term n m k} {t0 : Term n' m k}
   (he : t0 = t.rename f)
@@ -188,6 +193,8 @@ theorem Term.rename_id {t : Term n m k} :
     simp [Term.rename, SType.rename_id, ih]
   case bindc ih =>
     simp [Term.rename, CaptureSet.rename_id, ih]
+  case boundary ih =>
+    simp [Term.rename, SType.rename_id, ih, FinFun.id_ext]
 
 theorem Term.trename_id {t : Term n m k} :
   t.trename FinFun.id = t := by
@@ -225,6 +232,8 @@ theorem Term.trename_id {t : Term n m k} :
     exact ih
   case unbox =>
     simp [Term.trename]
+  case boundary ih =>
+    simp [Term.trename, SType.trename_id, ih, FinFun.id_ext]
 
 theorem Term.crename_id {t : Term n m k} :
   t.crename FinFun.id = t := by
@@ -261,5 +270,8 @@ theorem Term.crename_id {t : Term n m k} :
     simp [CaptureSet.crename_id, FinFun.id_ext, ih]
   case unbox =>
     simp [Term.crename, CaptureSet.crename_id]
+  case boundary ih =>
+    simp [Term.crename]
+    simp [ih, SType.crename_id, FinFun.id_ext]
 
 end Capless
